Added examples "append" and "reverse" as presented in Matthew Parkinsons lecture. The append example with data triggered a problem with the order of case-splitting that got fixed. Moreover, some minor tweaks to the proof of "insertionsort".

examples/separationLogic/src/vars_as_resourceFunctor.sml
@@ -1350,6 +1350,24 @@ in
 end;
 
 
+(* while preparing for the introduction of a "VAR_RES_FRAME_SPLIT" 
+   predicate, existential quantifiers are moved to the outer level.
+   This may cause trouble, because the choices for these variables have to
+   hold under all other (later) case-splits. Therefore, obvious case splits
+   are done first, like ones acoording to if-then-else. Moreover, 
+   concrete values for variables are introduced as well before the existential
+   quantifiers. *)
+
+fun VAR_RES_COND_INFERENCE___PREPARE_FOR_FRAME___CONV tt =
+let
+   val (_, pre, _, _) = dest_VAR_RES_COND_HOARE_TRIPLE tt;
+   fun not_ok t = is_cond t orelse is_var_res_prop_binexpression_cond t
+   val is_ok = (find_term not_ok pre; false) handle HOL_ERR _ => true;
+   val _ = if (is_ok) then () else Feedback.fail();
+in
+   VAR_RES_COND_INFERENCE___ALL_CONST_INTRO___CONV tt
+end;
+
 
 (*
    val tt = find_term is_VAR_RES_FRAME_SPLIT (snd (top_goal ()))
@@ -1389,7 +1407,7 @@ let
 
    (*elim comment / intro constants *)
    val thm0 = (((RATOR_CONV o RAND_CONV o RAND_CONV) (K (bl_eq_fun ()))) THENC
-               VAR_RES_COND_INFERENCE___ALL_CONST_INTRO___CONV) tt
+               VAR_RES_COND_INFERENCE___PREPARE_FOR_FRAME___CONV) tt
    val (vs, tt') = strip_forall (rhs (concl thm0))
 
    (*elim existentials in post-condition*)
@@ -1439,7 +1457,7 @@ let
 
     (*introduce constants*)
     val thm_const = CONV_RULE (RHS_CONV
-         VAR_RES_COND_INFERENCE___ALL_CONST_INTRO___CONV) (thm0_fun())
+         VAR_RES_COND_INFERENCE___PREPARE_FOR_FRAME___CONV) (thm0_fun())
     val (vs, tt') = strip_forall (rhs (concl thm_const))
 
 
@@ -1531,7 +1549,7 @@ let
 
     (*introduce constants*)
     val thm_const = CONV_RULE (RHS_CONV
-         VAR_RES_COND_INFERENCE___ALL_CONST_INTRO___CONV) (thm0_fun())
+         VAR_RES_COND_INFERENCE___PREPARE_FOR_FRAME___CONV) (thm0_fun())
     val (vs, tt') = strip_forall (rhs (concl thm_const))
 
 
@@ -1665,7 +1683,7 @@ let
 
     (*introduce constants*)
     val thm_const = CONV_RULE (RHS_CONV
-         VAR_RES_COND_INFERENCE___ALL_CONST_INTRO___CONV) (thm0_fun())
+         VAR_RES_COND_INFERENCE___PREPARE_FOR_FRAME___CONV) (thm0_fun())
     val (vs, tt') = strip_forall (rhs (concl thm_const))
 
 
@@ -1948,7 +1966,7 @@ let
    (*elim comment*)
    val thm0a = p1_thm_fun ();
    val thm0  = (VAR_RES_COND_HOARE_TRIPLE___FIRST_COMMAND___CONV (K thm0a)
-                THENC VAR_RES_COND_INFERENCE___ALL_CONST_INTRO___CONV) tt
+                THENC VAR_RES_COND_INFERENCE___PREPARE_FOR_FRAME___CONV) tt
    val (vs, tt') = strip_forall (rhs (concl thm0))
 
 
